theories/switcher/clear_registers_spec.v
@@ -6,7 +6,6 @@ From cap_machine Require Export cap_lang seal_store region_invariants.
 From iris.algebra Require Export gmap agree auth excl_auth.
 From iris.base_logic Require Export invariants na_invariants saved_prop.
 From cap_machine Require Import rules_base.
-From cap_machine Require Import rules_base clear_registers.
 From cap_machine Require Export clear_registers.
 
 
@@ -39,6 +38,101 @@ Section ClearRegistersMacro.
   Definition is_arg_rmap (rmap : Reg) (nargs : nat) :=
     dom rmap = dom_arg_rmap nargs.
 
+  Lemma rclear_spec
+    (pc_p : Perm) (pc_g : Locality) (pc_b pc_e pc_a : Addr)
+    (l : list RegName)
+    (rmap : Reg) φ :
+    l ≠ [] ->
+    executeAllowed pc_p = true ->
+    SubBounds pc_b pc_e pc_a (pc_a ^+ length (rclear_instrs' l ))%a ->
+
+    dom rmap = list_to_set l  ->
+
+    ( PC ↦ᵣ WCap pc_p pc_g pc_b pc_e pc_a
+      ∗ ( [∗ map] r↦w ∈ rmap, r ↦ᵣ w )
+      ∗ codefrag pc_a (rclear_instrs' l)
+      ∗ ▷ ( (∃ (rmap' : Reg),
+              ⌜ dom rmap' = list_to_set l ⌝
+              ∗ PC ↦ᵣ WCap pc_p pc_g pc_b pc_e (pc_a ^+ length (rclear_instrs' l ))%a
+              ∗ ( [∗ map] r↦w ∈ rmap', r ↦ᵣ w ∗ ⌜ w = WInt 0 ⌝ )
+              ∗ codefrag pc_a (rclear_instrs' l))
+               -∗ WP Seq (Instr Executable) {{ φ }})
+    )
+    ⊢ WP Seq (Instr Executable) {{ φ }}%I.
+  Proof.
+    iIntros (Hne Hx Hbounds Hdom) "(HPC & Hregs & Hcode & Hcont)".
+    iRevert (Hbounds Hdom).
+    iInduction (l) as [|r l] "IH" forall (rmap pc_a); iIntros (Hbounds Hrdom); first congruence.
+
+    cbn [list_to_set] in Hrdom.
+    assert (is_Some (rmap !! r)) as [rv Hr].
+    { apply elem_of_dom; rewrite Hrdom; set_solver. }
+    iDestruct (big_sepM_delete _ _ r with "Hregs") as "[Hr Hregs]"; eauto.
+    cbn.
+    codefrag_facts "Hcode".
+
+    iInstr "Hcode".
+    { transitivity (Some (pc_a ^+ 1)%a); auto; solve_addr. }
+    destruct (decide (l = [])).
+    { subst l. iApply "Hcont". iFrame.
+      replace (delete r rmap) with (∅ : Reg).
+      2: { symmetry.
+           rewrite -dom_empty_iff_L.
+           rewrite dom_delete_L.
+           rewrite Hrdom.
+           set_solver.
+         }
+      iExists (<[r := WInt 0]> ∅).
+      iSplit; cycle 1.
+      + iDestruct (big_sepM_insert (fun r w => r ↦ᵣ w ∗ ⌜ w = WInt 0⌝ )%I ∅ r with "[Hr Hregs]") as "H".
+        { done. }
+        { iFrame. iSplit; done. }
+        iFrame "H".
+      + iPureIntro ; set_solver.
+    }
+
+   iAssert (codefrag (pc_a ^+ 1)%a (rclear_instrs' l) ∗
+             (codefrag (pc_a ^+ 1)%a (rclear_instrs' l) -∗ codefrag pc_a (rclear_instrs' (r :: l))))%I
+    with "[Hcode]" as "[Hcode Hcls]".
+    { cbn. unfold codefrag. rewrite (region_pointsto_cons _ (pc_a ^+ 1)%a). 2,3: solve_addr.
+      iDestruct "Hcode" as "[? Hr]".
+      rewrite (_: ((pc_a ^+ 1) ^+ (length (rclear_instrs' l)))%a =
+                    (pc_a ^+ (S (length (rclear_instrs' l))))%a). 2: solve_addr.
+      iFrame. eauto. }
+
+    match goal with H : SubBounds _ _ _ _ |- _ =>
+      rewrite (_: (pc_a ^+ (length (rclear_instrs' (r :: l))))%a =
+                  ((pc_a ^+ 1)%a ^+ length (rclear_instrs' l))%a) in H |- *
+    end.
+    2: { unfold rclear_instrs'; cbn; solve_addr. }
+
+    destruct (decide (r ∈ l)).
+    - iDestruct (big_sepM_insert _ _ r with "[Hr $Hregs]") as "Hregs".
+      { by rewrite lookup_delete//. }
+      { by iFrame. }
+      iApply ("IH" with "[] HPC Hregs Hcode [Hcont Hcls]"); eauto.
+      { iNext.
+        iIntros "H"; iDestruct "H" as (rmap' Hdom_rmap')  "(HPC & Hregs & Hcode)".
+        iApply "Hcont"; iFrame.
+        iDestruct ("Hcls" with "Hcode") as "$".
+        iPureIntro; set_solver.
+      }
+      { iPureIntro; solve_pure_addr. }
+      {  iPureIntro. rewrite insert_delete_insert. set_solver. }
+    - iApply ("IH" with "[] HPC Hregs Hcode [Hcont Hcls Hr]"); eauto.
+      { iNext.
+        iIntros "H"; iDestruct "H" as (rmap' Hdom_rmap')  "(HPC & Hregs & Hcode)".
+        iDestruct (big_sepM_insert _ _ r with "[Hr $Hregs]") as "Hregs".
+        { rewrite -not_elem_of_dom Hdom_rmap'; set_solver. }
+        { iFrame. done. }
+        iApply "Hcont"; iFrame.
+        iDestruct ("Hcls" with "Hcode") as "$".
+        iPureIntro; set_solver.
+      }
+      { iPureIntro; solve_pure_addr. }
+      {  iPureIntro; set_solver. }
+  Qed.
+
   Lemma clear_registers_post_call_spec
     (pc_p : Perm) (pc_g : Locality) (pc_b pc_e pc_a : Addr)
     (rmap : Reg) φ :
@@ -60,50 +154,33 @@ Section ClearRegistersMacro.
     ⊢ WP Seq (Instr Executable) {{ φ }}%I.
   Proof.
     iIntros (Hx Hbounds Hdom) "(HPC & Hregs & Hcode & Hcont)".
-
-    iAssert ([∗ map] r↦_ ∈ rmap, ∃ w, r ↦ᵣ w)%I with "[Hregs]" as "Hregs".
-    { iApply (big_sepM_mono with "Hregs"). intros. eauto. }
-
-    iDestruct (big_sepM_dom with "Hregs") as "Hregs".
-    rewrite Hdom.
-
-    iDestruct (big_sepS_delete _ _ ct0 with "Hregs") as "[[% ?] Hregs]";[set_solver|].
-    iDestruct (big_sepS_delete _ _ cnull with "Hregs") as "[[% ?] Hregs]";[set_solver|].
-    iDestruct (big_sepS_delete _ _ ctp with "Hregs") as "[[% ?] Hregs]";[set_solver|].
-    iDestruct (big_sepS_delete _ _ ct1 with "Hregs") as "[[% ?] Hregs]";[set_solver|].
-    iDestruct (big_sepS_delete _ _ ct2 with "Hregs") as "[[% ?] Hregs]";[set_solver|].
-    iDestruct (big_sepS_delete _ _ ct3 with "Hregs") as "[[% ?] Hregs]";[set_solver|].
-    iDestruct (big_sepS_delete _ _ ct4 with "Hregs") as "[[% ?] Hregs]";[set_solver|].
-    iDestruct (big_sepS_delete _ _ ct5 with "Hregs") as "[[% ?] Hregs]";[set_solver|].
-    iDestruct (big_sepS_delete _ _ ct6 with "Hregs") as "[[% ?] Hregs]";[set_solver|].
-    iDestruct (big_sepS_delete _ _ ca2 with "Hregs") as "[[% ?] Hregs]";[set_solver|].
-    iDestruct (big_sepS_delete _ _ ca3 with "Hregs") as "[[% ?] Hregs]";[set_solver|].
-    iDestruct (big_sepS_delete _ _ ca4 with "Hregs") as "[[% ?] Hregs]";[set_solver|].
-    iDestruct (big_sepS_delete _ _ ca5 with "Hregs") as "[[% ?] Hregs]";[set_solver|].
-    iDestruct (big_sepS_delete _ _ ca6 with "Hregs") as "[[% ?] Hregs]";[set_solver|].
-    iDestruct (big_sepS_delete _ _ ca7 with "Hregs") as "[[% ?] Hregs]";[set_solver|].
-    iDestruct (big_sepS_delete _ _ cs2 with "Hregs") as "[[% ?] Hregs]";[set_solver|].
-    iDestruct (big_sepS_delete _ _ cs3 with "Hregs") as "[[% ?] Hregs]";[set_solver|].
-    iDestruct (big_sepS_delete _ _ cs4 with "Hregs") as "[[% ?] Hregs]";[set_solver|].
-    iDestruct (big_sepS_delete _ _ cs5 with "Hregs") as "[[% ?] Hregs]";[set_solver|].
-    iDestruct (big_sepS_delete _ _ cs6 with "Hregs") as "[[% ?] Hregs]";[set_solver|].
-    iDestruct (big_sepS_delete _ _ cs7 with "Hregs") as "[[% ?] Hregs]";[set_solver|].
-    iDestruct (big_sepS_delete _ _ cs8 with "Hregs") as "[[% ?] Hregs]";[set_solver|].
-    iDestruct (big_sepS_delete _ _ cs9 with "Hregs") as "[[% ?] Hregs]";[set_solver|].
-    iDestruct (big_sepS_delete _ _ cs10 with "Hregs") as "[[% ?] Hregs]";[set_solver|].
-    iDestruct (big_sepS_delete _ _ cs11 with "Hregs") as "[[% ?] _]";[set_solver|].
-
-    codefrag_facts "Hcode". clear H0.
-    iGo "Hcode".
-
-    iApply "Hcont".
-    iExists
-      (<[ct0:=_]> (<[cnull:=_]> (<[ctp:=_]> (<[ct1:=_]>(<[ct2:=_]>(<[ct3:=_]>(<[ct4:=_]>(<[ct5:=_]>(<[ct6:=_]>(<[ca2:=_]>(<[ca3:=_]>(<[ca4:=_]>(<[ca5:=_]>(<[ca6:=_]>(<[ca7:=_]> (<[cs2:=_]> (<[cs3:=_]> (<[cs4:=_]> (<[cs5:=_]> (<[cs6:=_]> (<[cs7:=_]> (<[cs8:=_]> (<[cs9:=_]> (<[cs10:=_]> (<[cs11:=_]> ∅))))))))))))))))))))))))).
-    repeat (rewrite big_sepM_insert;[|by simplify_map_eq]).
-    iFrame. iSplit.
-    { iPureIntro. rewrite !dom_insert_L. set_solver. }
-    repeat (iSplit;[done|]). done.
+    iApply (rclear_spec _ _ _ _ _ registers_post_call); eauto.
+    iFrame.
   Qed.
 
+  Lemma clear_registers_pre_call_spec
+    (pc_p : Perm) (pc_g : Locality) (pc_b pc_e pc_a : Addr)
+    (rmap : Reg) φ :
+    executeAllowed pc_p = true ->
+    SubBounds pc_b pc_e pc_a (pc_a ^+ length clear_registers_pre_call_instrs)%a ->
+
+    dom rmap = all_registers_s ∖ (dom_arg_rmap 8 ∪ {[ PC ; cra ; cgp ; csp ]}) ->
+
+    ( PC ↦ᵣ WCap pc_p pc_g pc_b pc_e pc_a
+      ∗ ( [∗ map] r↦w ∈ rmap, r ↦ᵣ w )
+      ∗ codefrag pc_a clear_registers_pre_call_instrs
+      ∗ ▷ ( (∃ (rmap' : Reg),
+              ⌜ dom rmap' = all_registers_s ∖ (dom_arg_rmap 8 ∪ {[ PC ; cra ; cgp ; csp ]}) ⌝
+              ∗ PC ↦ᵣ WCap pc_p pc_g pc_b pc_e (pc_a ^+ length clear_registers_pre_call_instrs)%a
+              ∗ ( [∗ map] r↦w ∈ rmap', r ↦ᵣ w ∗ ⌜ w = WInt 0 ⌝ )
+              ∗ codefrag pc_a clear_registers_pre_call_instrs)
+               -∗ WP Seq (Instr Executable) {{ φ }})
+    )
+    ⊢ WP Seq (Instr Executable) {{ φ }}%I.
+  Proof.
+    iIntros (Hx Hbounds Hdom) "(HPC & Hregs & Hcode & Hcont)".
+    iApply (rclear_spec _ _ _ _ _ registers_pre_call); eauto.
+    iFrame.
+  Qed.
 
 End ClearRegistersMacro.
